Tables.v
@@ -1,8 +1,8 @@
 Require Import String.
-Require Import FSets.FMapWeakList.
-Require Import FSets.FMapInterface.
-Require Import FSets.FMapFacts.
-Require Import Logic.DecidableType.
+Require Import FMapWeakList.
+Require Import FMapInterface.
+Require Import FMapFacts.
+Require Import DecidableType.
 
 Module StrDec : DecidableType
     with Definition t := string
@@ -41,46 +41,49 @@ Definition empty t := Table.empty t.
 Axiom Extensionality_Table : forall (t : Type) (A B : table t),
    Table.Equal A B -> A = B.
 
+Lemma equal_ind : forall (t : Type) A B,
+ (forall k (e : t), Table.MapsTo k e A -> Table.MapsTo k e B) ->
+ (forall k (e : t), Table.MapsTo k e B -> Table.MapsTo k e A) ->
+ A = B.
+Proof.
+intros.
+apply Extensionality_Table.
+apply (TableWF.Equal_mapsto_iff A B).
+split.
+ apply H.
+
+ apply H0.
+Qed.
+
 Lemma add_1 : forall (t : Type) (A : table t) x r1 r2,
   Table.add x r1 (Table.add x r2 A) = Table.add x r1 A.
 Proof.
 intros.
-apply Extensionality_Table.
-apply
- (TableWF.Equal_mapsto_iff (Table.add x r1 (Table.add x r2 A)) (Table.add x r1 A)).
- (* Table.MapsTo k e (Table.add y r1 (Table.add y r2 tenv)) ->
-    Table.MapsTo k e (Table.add y r1 tenv) *)
-split.
+apply equal_ind.
  intros.
  apply TableWF.add_mapsto_iff in H.
  decompose [or] H.
-  (* k = y *)
   inversion H0.
   rewrite H1 in |- *.
   rewrite H2 in |- *.
   apply Table.add_1.
   reflexivity.
 
-  (* k <> y *)
   decompose [and] H0.
   apply Table.add_2.
    trivial.
 
    apply Table.add_3 in H2; trivial.
 
- (* Table.MapsTo k e (Table.add y r1 tenv) ->
-    Table.MapsTo k e (Table.add y r1 (Table.add y r2 tenv)) *)
  intros.
  apply TableWF.add_mapsto_iff in H.
  decompose [or] H.
-  (* k = y *)
   inversion H0.
   rewrite H1 in |- *.
   rewrite H2 in |- *.
   apply Table.add_1.
   reflexivity.
 
-  (* k <> y *)
   inversion H0.
   apply Table.add_2.
    trivial.
@@ -92,73 +95,122 @@ Lemma add_2 : forall (t : Type) (A : table t) x y r1 r2,
   x <> y -> Table.add x r1 (Table.add y r2 A) = Table.add y r2 (Table.add x r1 A).
 Proof.
 intros.
-apply Extensionality_Table.
-apply
- (TableWF.Equal_mapsto_iff (Table.add x r1 (Table.add y r2 A))
-                           (Table.add y r2 (Table.add x r1 A))).
-split.
+apply equal_ind.
  intros.
  apply TableWF.add_mapsto_iff in H0.
- decompose [or] H0.
-  (* k = x *)
+ inversion H0.
   inversion H1.
   rewrite H2 in |- *.
   rewrite H3 in |- *.
-  rewrite H2 in H.
   apply Table.add_2.
    apply sym_not_eq.
+   rewrite <- H2.
    trivial.
 
    apply Table.add_1.
    reflexivity.
 
-  (* k <> x*)
   decompose [and] H1.
   apply TableWF.add_mapsto_iff in H3.
   decompose [or] H3.
-   (* y = k*)
    inversion H4.
    rewrite H5 in |- *; rewrite H6 in |- *.
    apply Table.add_1.
    reflexivity.
 
-   (* y <> k *)
    decompose [and] H4.
    apply Table.add_2.
     trivial.
 
     apply Table.add_2; trivial.
 
- (* Table.MapsTo k e (Table.add y r2 (Table.add x r1 tenv)) ->
-    Table.MapsTo k e (Table.add x r1 (Table.add y r2 tenv)) *)
  intros.
  apply TableWF.add_mapsto_iff in H0.
  decompose [or] H0.
-  (* k = y *)
   inversion H1.
   rewrite H2 in |- *; rewrite H3 in |- *.
-  rewrite H2 in H.
   apply Table.add_2.
+   trivial.
+   inversion H1.
+   decompose [or] H3.
+   inversion H4.
+   decompose [and] H4.
+   trivial.
+
+   rewrite <- H6.
    trivial.
 
    apply Table.add_1.
    reflexivity.
 
-  (* k <> y *)
   inversion H1.
   apply TableWF.add_mapsto_iff in H3.
   decompose [or] H3.
-   (* k = x *)
    inversion H4.
    rewrite H6 in |- *.
    rewrite H5 in |- *.
    apply Table.add_1.
    reflexivity.
 
-   (* k <> x *)
    decompose [and] H4.
    apply Table.add_2.
     trivial.
 
     apply Table.add_2; trivial.
+Qed.
+
+Lemma map_add : forall (A : Type) (f : A -> A) x T table,
+  Table.map f (Table.add x T table) = Table.add x (f T) (Table.map f table).
+Proof.
+intros.
+apply equal_ind.
+ intros.
+ apply TableWF.map_mapsto_iff in H.
+ inversion H.
+ inversion H0.
+ apply TableWF.add_mapsto_iff in H2.
+ inversion H2.
+  inversion H3.
+  rewrite H4 in |- *.
+  rewrite H5 in |- *.
+  rewrite H1 in |- *.
+  apply Table.add_1.
+  reflexivity.
+
+  inversion H3.
+  apply Table.add_2.
+   trivial.
+
+   apply (TableWF.map_mapsto_iff table0 k e f).
+   exists x0.
+   split.
+    trivial.
+
+    trivial.
+
+ intros.
+ apply TableWF.add_mapsto_iff in H.
+ apply (TableWF.map_mapsto_iff (Table.add x T table0) k e f).
+ inversion H.
+  inversion H0.
+  exists T.
+  split.
+   rewrite H2 in |- *.
+   reflexivity.
+
+   apply Table.add_1.
+   trivial.
+
+  inversion H0.
+  apply (TableWF.map_mapsto_iff table0 k e f) in H2.
+  inversion H2.
+  inversion H3.
+  exists x0.
+  split.
+   trivial.
+
+   apply Table.add_2.
+    trivial.
+
+    trivial.
 Qed.
